update faucet and token contract

src/ContractExamples/Faucet.fst
@@ -3,39 +3,48 @@ open Zen.Vector
 open Zen.Base
 open Zen.Cost
 open Zen.Asset
-open FStar.Mul
-        
+
+module E = Zen.Error
 module ET = Zen.ErrorT
 module Tx = Zen.TxSkeleton
 
-val cf: txSkeleton -> string -> data -> option lock -> #l:nat -> wallet l -> cost nat 11
-let cf _ _ _ _ #l _ = 
-    ret (64 + l * 128 + 192 + 15 + 9)
-          
-let get #l txSkeleton contractHash returnAddress (wallet:wallet l) =  
+val cf: txSkeleton -> string -> data -> option lock -> #l:nat -> wallet l -> cost nat 13
+let cf _ _ _ _ #l _ =
+    ret (64 + (l * 128 + 192) + 15 + 9 + 11)
+
+val withNoContract: result txSkeleton -> cost (result (txSkeleton ** option message)) 9
+let withNoContract result =
+    match result with
+    | OK txSkeleton -> ET.ret (txSkeleton,None)
+    | EX e -> ET.autoFail e
+    | ERR msg -> ET.autoFailw msg
+
+val get: #l:nat -> txSkeleton -> contractHash -> option lock -> wallet l -> cost (result txSkeleton) (64 + (l * 128 + 192) + 15)
+let get #l txSkeleton contractHash returnAddress (wallet:wallet l) =
   match returnAddress with
-  | Some returnAddress ->         
-      let txSkeleton = 
+  | Some returnAddress ->
+      let txSkeleton =
         Tx.lockToAddress zenAsset 10000UL returnAddress txSkeleton
         >>= Tx.fromWallet zenAsset 10000UL contractHash wallet in
-        
+
       ET.of_optionT "contract doesn't have enough zens to pay you" txSkeleton
   | None ->
       ET.autoFailw "returnAddress is required"
-    
-let init txSkeleton contractHash  = 
+
+val init: txSkeleton -> contractHash -> cost (result txSkeleton) (64 + 64 + 8)
+let init txSkeleton contractHash  =
   let! tokens = Tx.getAvailableTokens zenAsset txSkeleton in
 
   let txSkeleton = Tx.lockToContract zenAsset tokens contractHash txSkeleton in
-  ET.retT txSkeleton  
-  
-val main: txSkeleton -> hash -> string -> data -> option lock -> #l:nat -> wallet l -> cost (result txSkeleton) (64 + l * 128 + 192 + 15 + 9)
-let main txSkeleton contractHash command data returnAddress #l wallet =  
+  ET.retT txSkeleton
+
+val main: txSkeleton -> hash -> string -> data -> option lock -> #l:nat -> wallet l -> cost (result (txSkeleton ** option message))  (64 + (l * 128 + 192) + 15 + 9 + 11)
+let main txSkeleton contractHash command data returnAddress #l wallet =
   if command <> "init" then
     get txSkeleton contractHash returnAddress wallet
+    >>= withNoContract
+
   else
-    init txSkeleton contractHash     
-    |> autoInc
-  
-  
- 
+    autoInc (init txSkeleton contractHash >>= withNoContract)
+
+
